<?xml version="1.0"?>
<rdf:RDF xmlns="http://purl.obolibrary.org/obo/cro.owl#"
     xml:base="http://purl.obolibrary.org/obo/cro.owl"
     xmlns:rdf="http://www.w3.org/1999/02/22-rdf-syntax-ns#"
     xmlns:owl="http://www.w3.org/2002/07/owl#"
     xmlns:xml="http://www.w3.org/XML/1998/namespace"
     xmlns:xsd="http://www.w3.org/2001/XMLSchema#"
     xmlns:rdfs="http://www.w3.org/2000/01/rdf-schema#">
    <owl:Ontology rdf:about="http://purl.obolibrary.org/obo/cro.owl"/>
    


    <!-- 
    ///////////////////////////////////////////////////////////////////////////////////////
    //
    // Classes
    //
    ///////////////////////////////////////////////////////////////////////////////////////
     -->

    


    <!-- http://purl.obolibrary.org/obo/cro.owl#CRO_0000000 -->

    <owl:Class rdf:about="http://purl.obolibrary.org/obo/cro.owl#CRO_0000000">
        <rdfs:subClassOf rdf:resource="http://www.w3.org/2002/07/owl#Thing"/>
        <rdfs:label>Contribution Role</rdfs:label>
    </owl:Class>
    


    <!-- http://purl.obolibrary.org/obo/cro.owl#CRO_0000001 -->

    <owl:Class rdf:about="http://purl.obolibrary.org/obo/cro.owl#CRO_0000001">
        <rdfs:subClassOf rdf:resource="http://purl.obolibrary.org/obo/cro.owl#CRO_0000000"/>
        <rdfs:comment>Contributions to the research team and project.</rdfs:comment>
        <rdfs:label>Research Team Contribution Role</rdfs:label>
    </owl:Class>
    


    <!-- http://purl.obolibrary.org/obo/cro.owl#CRO_0000002 -->

    <owl:Class rdf:about="http://purl.obolibrary.org/obo/cro.owl#CRO_0000002">
        <rdfs:subClassOf rdf:resource="http://purl.obolibrary.org/obo/cro.owl#CRO_0000000"/>
        <rdfs:comment>Contributions to the published research object</rdfs:comment>
        <rdfs:label>Research Object Contribution Role</rdfs:label>
    </owl:Class>
    


    <!-- http://purl.obolibrary.org/obo/cro.owl#CRO_0000003 -->

    <owl:Class rdf:about="http://purl.obolibrary.org/obo/cro.owl#CRO_0000003">
        <rdfs:subClassOf rdf:resource="http://purl.obolibrary.org/obo/cro.owl#CRO_0000001"/>
        <rdfs:comment>Ideas; formulation or evolution of overarching research goals and aims.</rdfs:comment>
        <rdfs:label>Conceptualization Role</rdfs:label>
    </owl:Class>
    


    <!-- http://purl.obolibrary.org/obo/cro.owl#CRO_0000004 -->

    <owl:Class rdf:about="http://purl.obolibrary.org/obo/cro.owl#CRO_0000004">
        <rdfs:subClassOf rdf:resource="http://purl.obolibrary.org/obo/cro.owl#CRO_0000001"/>
        <rdfs:comment>Development or design of methodology; creation of models.</rdfs:comment>
        <rdfs:label>Methodology Role</rdfs:label>
    </owl:Class>
    


    <!-- http://purl.obolibrary.org/obo/cro.owl#CRO_0000005 -->

    <owl:Class rdf:about="http://purl.obolibrary.org/obo/cro.owl#CRO_0000005">
        <rdfs:subClassOf rdf:resource="http://purl.obolibrary.org/obo/cro.owl#CRO_0000001"/>
        <rdfs:comment>Programming, software development; designing computer programs; implementation of the computer code and supporting algorithms; testing of existing code components.</rdfs:comment>
        <rdfs:label>Software Development Role</rdfs:label>
    </owl:Class>
    


    <!-- http://purl.obolibrary.org/obo/cro.owl#CRO_0000006 -->

    <owl:Class rdf:about="http://purl.obolibrary.org/obo/cro.owl#CRO_0000006">
        <rdfs:subClassOf rdf:resource="http://purl.obolibrary.org/obo/cro.owl#CRO_0000001"/>
        <rdfs:comment>Verification, whether as a part of the activity or separate, of the overall replication/reproducibility of results/experiments and other research outputs.</rdfs:comment>
        <rdfs:label>Validation Role</rdfs:label>
    </owl:Class>
    


    <!-- http://purl.obolibrary.org/obo/cro.owl#CRO_0000007 -->

    <owl:Class rdf:about="http://purl.obolibrary.org/obo/cro.owl#CRO_0000007">
        <rdfs:subClassOf rdf:resource="http://purl.obolibrary.org/obo/cro.owl#CRO_0000001"/>
        <rdfs:comment>Application of statistical, mathematical, computational, or other formal techniques to analyse or synthesize study data.</rdfs:comment>
        <rdfs:label>Formal Analysis Role</rdfs:label>
    </owl:Class>
    


    <!-- http://purl.obolibrary.org/obo/cro.owl#CRO_0000008 -->

    <owl:Class rdf:about="http://purl.obolibrary.org/obo/cro.owl#CRO_0000008">
        <rdfs:subClassOf rdf:resource="http://purl.obolibrary.org/obo/cro.owl#CRO_0000001"/>
        <rdfs:comment>Conducting a research and investigation process, specifically performing the experiments, or data/evidence collection.</rdfs:comment>
        <rdfs:label>Investigation Role</rdfs:label>
    </owl:Class>
    


    <!-- http://purl.obolibrary.org/obo/cro.owl#CRO_0000009 -->

    <owl:Class rdf:about="http://purl.obolibrary.org/obo/cro.owl#CRO_0000009">
        <rdfs:subClassOf rdf:resource="http://purl.obolibrary.org/obo/cro.owl#CRO_0000001"/>
        <rdfs:comment>Provision of study materials, reagents, materials, patients, laboratory samples, animals, instrumentation, computing resources, or other analysis tools.</rdfs:comment>
        <rdfs:label>Resource Provision Role</rdfs:label>
    </owl:Class>
    


    <!-- http://purl.obolibrary.org/obo/cro.owl#CRO_0000010 -->

    <owl:Class rdf:about="http://purl.obolibrary.org/obo/cro.owl#CRO_0000010">
        <rdfs:subClassOf rdf:resource="http://purl.obolibrary.org/obo/cro.owl#CRO_0000001"/>
        <rdfs:comment>Management activities to annotate (produce metadata), scrub data and maintain research data (including software code, where it is necessary for interpreting the data itself) for initial use and later re-use.</rdfs:comment>
        <rdfs:label>Data Curation Role</rdfs:label>
    </owl:Class>
    


    <!-- http://purl.obolibrary.org/obo/cro.owl#CRO_0000011 -->

    <owl:Class rdf:about="http://purl.obolibrary.org/obo/cro.owl#CRO_0000011">
        <rdfs:subClassOf rdf:resource="http://purl.obolibrary.org/obo/cro.owl#CRO_0000001"/>
        <rdfs:comment>Oversight and leadership responsibility for the research activity planning and execution, including mentorship external to the core team.</rdfs:comment>
        <rdfs:label>Supervision Role</rdfs:label>
    </owl:Class>
    


    <!-- http://purl.obolibrary.org/obo/cro.owl#CRO_0000012 -->

    <owl:Class rdf:about="http://purl.obolibrary.org/obo/cro.owl#CRO_0000012">
        <rdfs:subClassOf rdf:resource="http://purl.obolibrary.org/obo/cro.owl#CRO_0000001"/>
        <rdfs:comment>Management and coordination responsibility for the research activity planning and execution.</rdfs:comment>
        <rdfs:label>Project Administration Role</rdfs:label>
    </owl:Class>
    


    <!-- http://purl.obolibrary.org/obo/cro.owl#CRO_0000013 -->

    <owl:Class rdf:about="http://purl.obolibrary.org/obo/cro.owl#CRO_0000013">
        <rdfs:subClassOf rdf:resource="http://purl.obolibrary.org/obo/cro.owl#CRO_0000001"/>
        <rdfs:comment>Acquisition of the financial support for the project leading to this publication.</rdfs:comment>
        <rdfs:label>Funding Acquisition Role</rdfs:label>
    </owl:Class>
    


    <!-- http://purl.obolibrary.org/obo/cro.owl#CRO_0000014 -->

    <owl:Class rdf:about="http://purl.obolibrary.org/obo/cro.owl#CRO_0000014">
        <rdfs:subClassOf rdf:resource="http://purl.obolibrary.org/obo/cro.owl#CRO_0000001"/>
        <rdfs:comment>Coordination of diverse team members, often across different disciplines and locations.</rdfs:comment>
        <rdfs:label>Team Management Role</rdfs:label>
    </owl:Class>
    


    <!-- http://purl.obolibrary.org/obo/cro.owl#CRO_0000015 -->

    <owl:Class rdf:about="http://purl.obolibrary.org/obo/cro.owl#CRO_0000015">
        <rdfs:subClassOf rdf:resource="http://purl.obolibrary.org/obo/cro.owl#CRO_0000001"/>
        <rdfs:comment>Manual entry or automated ingestion.</rdfs:comment>
        <rdfs:label>Data Entry Role</rdfs:label>
    </owl:Class>
    


    <!-- http://purl.obolibrary.org/obo/cro.owl#CRO_0000016 -->

    <owl:Class rdf:about="http://purl.obolibrary.org/obo/cro.owl#CRO_0000016">
        <rdfs:subClassOf rdf:resource="http://purl.obolibrary.org/obo/cro.owl#CRO_0000001"/>
        <rdfs:comment>Coordination of research dissemination through popular media and the press, as well as Community Outreach and liaising of project directly to the community.</rdfs:comment>
        <rdfs:label>Science Communication Role</rdfs:label>
    </owl:Class>
    


    <!-- http://purl.obolibrary.org/obo/cro.owl#CRO_0000017 -->

    <owl:Class rdf:about="http://purl.obolibrary.org/obo/cro.owl#CRO_0000017">
        <rdfs:subClassOf rdf:resource="http://purl.obolibrary.org/obo/cro.owl#CRO_0000001"/>
        <rdfs:comment>Includes literature searches and contributions to review activities (systematic reviews, scoping reviews, etc.)</rdfs:comment>
        <rdfs:label>Background and Literature Search Role</rdfs:label>
    </owl:Class>
    


    <!-- http://purl.obolibrary.org/obo/cro.owl#CRO_0000018 -->

    <owl:Class rdf:about="http://purl.obolibrary.org/obo/cro.owl#CRO_0000018">
        <rdfs:subClassOf rdf:resource="http://purl.obolibrary.org/obo/cro.owl#CRO_0000001"/>
        <rdfs:comment>Manage regulatory and compliance issues for the research project.</rdfs:comment>
        <rdfs:label>Regulatory Administration Role</rdfs:label>
    </owl:Class>
    


    <!-- http://purl.obolibrary.org/obo/cro.owl#CRO_0000019 -->

    <owl:Class rdf:about="http://purl.obolibrary.org/obo/cro.owl#CRO_0000019">
        <rdfs:subClassOf rdf:resource="http://purl.obolibrary.org/obo/cro.owl#CRO_0000002"/>
        <rdfs:comment>Preparation, creation and/or presentation of the published work, specifically writing the initial draft (including substantive translation).</rdfs:comment>
        <rdfs:label>Writing Original Draft Role</rdfs:label>
    </owl:Class>
    


    <!-- http://purl.obolibrary.org/obo/cro.owl#CRO_0000020 -->

    <owl:Class rdf:about="http://purl.obolibrary.org/obo/cro.owl#CRO_0000020">
        <rdfs:subClassOf rdf:resource="http://purl.obolibrary.org/obo/cro.owl#CRO_0000002"/>
        <rdfs:comment>Preparation, creation and/or presentation of the published work by those from the original research group, specifically critical review, commentary or revision – including pre- or post-publication stages.</rdfs:comment>
        <rdfs:label>Reviewing and Editing Manuscript Role</rdfs:label>
    </owl:Class>
    


    <!-- http://purl.obolibrary.org/obo/cro.owl#CRO_0000021 -->

    <owl:Class rdf:about="http://purl.obolibrary.org/obo/cro.owl#CRO_0000021">
        <rdfs:subClassOf rdf:resource="http://purl.obolibrary.org/obo/cro.owl#CRO_0000002"/>
        <rdfs:comment>Preparation, creation and/or presentation of the published work, specifically visualization/data presentation.</rdfs:comment>
        <rdfs:label>Visualization Role</rdfs:label>
    </owl:Class>
    


    <!-- http://purl.obolibrary.org/obo/cro.owl#CRO_0000022 -->

    <owl:Class rdf:about="http://purl.obolibrary.org/obo/cro.owl#CRO_0000022">
        <rdfs:subClassOf rdf:resource="http://purl.obolibrary.org/obo/cro.owl#CRO_0000002"/>
        <rdfs:comment>Coordination of the deposit of the manuscript, data, and any secondary materials to appropriate repositories; ensure that outputs comply with OA mandates.</rdfs:comment>
        <rdfs:label>Preservation Role</rdfs:label>
    </owl:Class>
</rdf:RDF>



<!-- Generated by the OWL API (version 4.1.3.20151118-2017) https://github.com/owlcs/owlapi -->

