Prefix(:=<http://purl.obolibrary.org/obo/cro.owl#>)
Prefix(cro:=<http://purl.obolibrary.org/obo/cro.owl#>)
Prefix(owl:=<http://www.w3.org/2002/07/owl#>)
Prefix(rdf:=<http://www.w3.org/1999/02/22-rdf-syntax-ns#>)
Prefix(xml:=<http://www.w3.org/XML/1998/namespace>)
Prefix(xsd:=<http://www.w3.org/2001/XMLSchema#>)
Prefix(rdfs:=<http://www.w3.org/2000/01/rdf-schema#>)


Ontology(<http://purl.obolibrary.org/obo/cro.owl>
Import(<http://vivoweb.org/ontology/core>)

Declaration(Class(:CRO_0000000))
Declaration(Class(:CRO_0000001))
Declaration(Class(:CRO_0000002))
Declaration(Class(:CRO_0000003))
Declaration(Class(:CRO_0000004))
Declaration(Class(:CRO_0000005))
Declaration(Class(:CRO_0000006))
Declaration(Class(:CRO_0000007))
Declaration(Class(:CRO_0000008))
Declaration(Class(:CRO_0000009))
Declaration(Class(:CRO_0000010))
Declaration(Class(:CRO_0000011))
Declaration(Class(:CRO_0000012))
Declaration(Class(:CRO_0000013))
Declaration(Class(:CRO_0000014))
Declaration(Class(:CRO_0000015))
Declaration(Class(:CRO_0000016))
Declaration(Class(:CRO_0000017))
Declaration(Class(:CRO_0000018))
Declaration(Class(:CRO_0000019))
Declaration(Class(:CRO_0000020))
Declaration(Class(:CRO_0000022))
Declaration(Class(:CRO_0000023))
Declaration(Class(:CRO_0000024))
Declaration(Class(:CRO_0000025))
Declaration(Class(:CRO_0000026))
Declaration(Class(:CRO_0000027))
Declaration(Class(:CRO_0000028))
Declaration(Class(:CRO_0000029))


############################
#   Classes
############################

# Class: :CRO_0000000 (Contribution Role)

AnnotationAssertion(<http://purl.obolibrary.org/obo/IAO_0000115> :CRO_0000000 "A high-level classification of the diverse roles performed in the work leading to a published research output in the sciences. Its purpose to provide transparency in contributions to scholarly published work, to enable improved systems of attribution, credit, and accountability.")
AnnotationAssertion(rdfs:label :CRO_0000000 "Contribution Role")
SubClassOf(:CRO_0000000 <http://purl.obolibrary.org/obo/BFO_0000023>)

# Class: :CRO_0000001 (Author Role)

AnnotationAssertion(<http://purl.obolibrary.org/obo/IAO_0000115> :CRO_0000001 "Contributions to the published research object")
AnnotationAssertion(rdfs:label :CRO_0000001 "Author Role")
SubClassOf(:CRO_0000001 :CRO_0000000)

# Class: :CRO_0000002 (Conceptualization Role)

AnnotationAssertion(<http://purl.obolibrary.org/obo/IAO_0000115> :CRO_0000002 "Ideas; formulation or evolution of overarching research goals and aims.")
AnnotationAssertion(rdfs:label :CRO_0000002 "Conceptualization Role")
SubClassOf(:CRO_0000002 :CRO_0000000)

# Class: :CRO_0000003 (Methodology Role)

AnnotationAssertion(<http://purl.obolibrary.org/obo/IAO_0000115> :CRO_0000003 "Development or design of methodology; creation of models.")
AnnotationAssertion(rdfs:label :CRO_0000003 "Methodology Role")
SubClassOf(:CRO_0000003 :CRO_0000000)

# Class: :CRO_0000004 (Software Development Role)

AnnotationAssertion(<http://purl.obolibrary.org/obo/IAO_0000115> :CRO_0000004 "Programming, software development; designing computer programs; implementation of the computer code and supporting algorithms; testing of existing code components.")
AnnotationAssertion(rdfs:label :CRO_0000004 "Software Development Role")
SubClassOf(:CRO_0000004 :CRO_0000000)

# Class: :CRO_0000005 (Validation Role)

AnnotationAssertion(<http://purl.obolibrary.org/obo/IAO_0000115> :CRO_0000005 "Verification, whether as a part of the activity or separate, of the overall replication/reproducibility of results/experiments and other research outputs.")
AnnotationAssertion(rdfs:label :CRO_0000005 "Validation Role")
SubClassOf(:CRO_0000005 :CRO_0000000)

# Class: :CRO_0000006 (Formal Analysis Role)

AnnotationAssertion(<http://purl.obolibrary.org/obo/IAO_0000115> :CRO_0000006 "Application of statistical, mathematical, computational, or other formal techniques to analyse or synthesize study data.")
AnnotationAssertion(rdfs:label :CRO_0000006 "Formal Analysis Role")
SubClassOf(:CRO_0000006 :CRO_0000000)

# Class: :CRO_0000007 (Investigation Role)

AnnotationAssertion(<http://purl.obolibrary.org/obo/IAO_0000115> :CRO_0000007 "Conducting a research and investigation process, specifically performing the experiments, or data/evidence collection.")
AnnotationAssertion(rdfs:label :CRO_0000007 "Investigation Role")
AnnotationAssertion(rdfs:label :CRO_0000007 "Research Investigation Role")
SubClassOf(:CRO_0000007 :CRO_0000000)

# Class: :CRO_0000008 (Resource Provision Role)

AnnotationAssertion(<http://purl.obolibrary.org/obo/IAO_0000115> :CRO_0000008 "Provision of study materials, reagents, materials, patients, laboratory samples, animals, instrumentation, computing resources, or other analysis tools.")
AnnotationAssertion(rdfs:label :CRO_0000008 "Resource Provision Role")
SubClassOf(:CRO_0000008 :CRO_0000000)

# Class: :CRO_0000009 (Data Curation Role)

AnnotationAssertion(<http://purl.obolibrary.org/obo/IAO_0000115> :CRO_0000009 "Management activities to annotate (produce metadata), scrub data and maintain research data (including software code, where it is necessary for interpreting the data itself) for initial use and later re-use.")
AnnotationAssertion(rdfs:label :CRO_0000009 "Data Curation Role")
SubClassOf(:CRO_0000009 :CRO_0000000)

# Class: :CRO_0000010 (Supervision Role)

AnnotationAssertion(<http://purl.obolibrary.org/obo/IAO_0000115> :CRO_0000010 "Oversight and leadership responsibility for the research activity planning and execution, including mentorship external to the core team.")
AnnotationAssertion(rdfs:label :CRO_0000010 "Supervision Role")
SubClassOf(:CRO_0000010 :CRO_0000000)

# Class: :CRO_0000011 (Project Administration Role)

AnnotationAssertion(<http://purl.obolibrary.org/obo/IAO_0000115> :CRO_0000011 "Management and coordination responsibility for the research activity planning and execution.")
AnnotationAssertion(rdfs:label :CRO_0000011 "Project Administration Role")
SubClassOf(:CRO_0000011 :CRO_0000000)

# Class: :CRO_0000012 (Funding Acquisition Role)

AnnotationAssertion(<http://purl.obolibrary.org/obo/IAO_0000115> :CRO_0000012 "Acquisition of the financial support for the project leading to this publication.")
AnnotationAssertion(rdfs:label :CRO_0000012 "Funding Acquisition Role")
SubClassOf(:CRO_0000012 :CRO_0000000)

# Class: :CRO_0000013 (Team Management Role)

AnnotationAssertion(<http://purl.obolibrary.org/obo/IAO_0000115> :CRO_0000013 "Coordination of diverse team members, often across different disciplines and locations.")
AnnotationAssertion(rdfs:label :CRO_0000013 "Team Management Role")
SubClassOf(:CRO_0000013 :CRO_0000000)

# Class: :CRO_0000014 (Data Entry Role)

AnnotationAssertion(<http://purl.obolibrary.org/obo/IAO_0000115> :CRO_0000014 "Manual entry or automated ingestion.")
AnnotationAssertion(rdfs:label :CRO_0000014 "Data Entry Role")
SubClassOf(:CRO_0000014 :CRO_0000000)

# Class: :CRO_0000015 (Science Communication Role)

AnnotationAssertion(<http://purl.obolibrary.org/obo/IAO_0000115> :CRO_0000015 "Coordination of research dissemination through popular media and the press, as well as Community Outreach and liaising of project directly to the community.")
AnnotationAssertion(rdfs:label :CRO_0000015 "Science Communication Role")
SubClassOf(:CRO_0000015 :CRO_0000000)

# Class: :CRO_0000016 (Background and Literature Search Role)

AnnotationAssertion(<http://purl.obolibrary.org/obo/IAO_0000115> :CRO_0000016 "Includes literature searches and contributions to review activities (systematic reviews, scoping reviews, etc.)")
AnnotationAssertion(rdfs:label :CRO_0000016 "Background and Literature Search Role")
SubClassOf(:CRO_0000016 :CRO_0000000)

# Class: :CRO_0000017 (Regulatory Administration Role)

AnnotationAssertion(<http://purl.obolibrary.org/obo/IAO_0000115> :CRO_0000017 "Manage regulatory and compliance issues for the research project.")
AnnotationAssertion(rdfs:label :CRO_0000017 "Regulatory Administration Role")
SubClassOf(:CRO_0000017 :CRO_0000000)

# Class: :CRO_0000018 (Data Visualization Role)

AnnotationAssertion(<http://purl.obolibrary.org/obo/IAO_0000115> :CRO_0000018 "Preparation, creation and/or presentation of the published work, specifically visualization/data presentation.")
AnnotationAssertion(rdfs:label :CRO_0000018 "Data Visualization Role")
SubClassOf(:CRO_0000018 :CRO_0000000)

# Class: :CRO_0000019 (Writing Original Draft Role)

AnnotationAssertion(<http://purl.obolibrary.org/obo/IAO_0000115> :CRO_0000019 "Preparation, creation and/or presentation of the published work, specifically writing the initial draft (including substantive translation).")
AnnotationAssertion(rdfs:label :CRO_0000019 "Writing Original Draft Role")
SubClassOf(:CRO_0000019 :CRO_0000001)

# Class: :CRO_0000020 (Reviewing and Editing Manuscript Role)

AnnotationAssertion(<http://purl.obolibrary.org/obo/IAO_0000115> :CRO_0000020 "Preparation, creation and/or presentation of the published work by those from the original research group, specifically critical review, commentary or revision â€“ including pre- or post-publication stages.")
AnnotationAssertion(rdfs:label :CRO_0000020 "Reviewing and Editing Manuscript Role")
SubClassOf(:CRO_0000020 :CRO_0000001)

# Class: :CRO_0000022 (Preservation Role)

AnnotationAssertion(<http://purl.obolibrary.org/obo/IAO_0000115> :CRO_0000022 "Coordination of the deposit of the manuscript, data, and any secondary materials to appropriate repositories; ensure that outputs comply with OA mandates.")
AnnotationAssertion(rdfs:label :CRO_0000022 "Preservation Role")
SubClassOf(:CRO_0000022 :CRO_0000001)

# Class: :CRO_0000023 (Computer Programming Role)

AnnotationAssertion(rdfs:label :CRO_0000023 "Computer Programming Role")
SubClassOf(:CRO_0000023 :CRO_0000004)

# Class: :CRO_0000024 (Software Architecture Role)

AnnotationAssertion(rdfs:label :CRO_0000024 "Software Architecture Role")
SubClassOf(:CRO_0000024 :CRO_0000004)

# Class: :CRO_0000025 (Software Design Role)

AnnotationAssertion(rdfs:label :CRO_0000025 "Software Design Role")
SubClassOf(:CRO_0000025 :CRO_0000004)

# Class: :CRO_0000026 (Software Engineering Role)

AnnotationAssertion(rdfs:label :CRO_0000026 "Software Engineering Role")
SubClassOf(:CRO_0000026 :CRO_0000004)

# Class: :CRO_0000027 (Software Testing Role)

AnnotationAssertion(rdfs:label :CRO_0000027 "Software Testing Role")
SubClassOf(:CRO_0000027 :CRO_0000004)

# Class: :CRO_0000028 (Quality Assurance Role)

AnnotationAssertion(rdfs:label :CRO_0000028 "Quality Assurance Role")
SubClassOf(:CRO_0000028 :CRO_0000004)

# Class: :CRO_0000029 (Technical Writing Role)

AnnotationAssertion(rdfs:label :CRO_0000029 "Technical Writing Role")
SubClassOf(:CRO_0000029 :CRO_0000004)


)